start proof 2

security/BacktranslationProof2.v
@@ -9,6 +9,7 @@ Require Import riscV.Asm.
 Require Import BtBasics BtInfoAsm MemoryDelta MemoryWeak.
 Require Import Ctypes Clight.
 Require Import Backtranslation BacktranslationAux BacktranslationProof.
+Require Import RSC.
 
 
 Section GENPROOFS.
@@ -62,3 +63,127 @@ End GENPROOFS.
 (*   forall [F V : Type] {CF : has_comp F} (ge : Genv.t F V) [thr : block], *)
 (*   (forall (id : ident) (b : block), Genv.find_symbol ge id = Some b -> Plt b thr) -> *)
 (*   forall (gl : list (ident * globdef F V)) (m m' : mem), Genv.alloc_globals ge m gl = Some m' -> Mem.inject_neutral thr m -> Ple (Mem.nextblock m') thr -> Mem.inject_neutral thr m' *)
+
+
+Section PROOFINIT.
+
+  Definition asm_program_does_prefix (p: Asm.program) (t: trace) :=
+    semantics_has_initial_trace_prefix (Asm.semantics p) t.
+  Definition clight_program_does_prefix (p: Clight.program) (t: trace) :=
+    semantics_has_initial_trace_prefix (Clight.semantics1 p) t.
+
+  (* Lemma behaves_star_prefix *)
+  (*       L beh *)
+  (*       (s: Smallstep.state L) *)
+  (*       (BEH: state_behaves L s beh) *)
+  (*       tr *)
+  (*       (PRE: behavior_prefix tr beh) *)
+  (*   : *)
+  (*   exists s', Star L s tr s'. *)
+  (* Proof. *)
+
+  (* Admitted. *)
+
+  Theorem asm_to_clight
+          (p: Asm.program) (ast: Asm.state)
+          (WFP: wf_program p)
+          (WFMAIN: wf_main p)
+          (WFMAINSIG: wf_main_sig p)
+          (WFINIT: exists (s : Asm.state), Asm.initial_state p s)
+    (* (WF: exists (s: Smallstep.state (semantics p)), Smallstep.initial_state (semantics p) s) *)
+    :
+    forall tr, asm_program_does_prefix p tr ->
+          exists btr,
+            clight_program_does_prefix (gen_program btr p) tr /\
+              unbundle_trace btr = tr.
+  Proof.
+    i. eapply semantics_has_initial_trace_prefix_implies_cut in H.
+    2:{ apply sd_traces. apply semantics_determinate. }
+    inv H; cycle 1.
+    { exfalso. ss. des. eapply H0. eapply WFINIT. }
+    clear WFINIT. ss. des. hexploit ir_has_initial_state; eauto. intros (ist & IR_INIT).
+    hexploit match_state_initial_state; eauto. intros (m0 & j & INIT_MEM_A & MS_I).
+    hexploit asm_to_ir.
+    { eapply wf_program_wf_ge; eauto. }
+    { eapply wf_asm_initial_state; eauto. }
+    { assert (star (step_fix (comp_of_main p)) (Genv.globalenv p) s tr s').
+      { admit. (* fix asm step *) }
+      eapply H.
+    }
+    { eapply MS_I. }
+    intros (btr & ist' & UTR & ISTAR). esplits. 2: eauto.
+    eapply semantics_has_initial_trace_cut_implies_prefix. econs 1; ss.
+
+    TODO
+
+    Lemma gen_program_exists_initial_state
+          (p: Asm.program) btr
+  (ist : ir_state)
+  (IR_INIT : ir_initial_state p ist)
+      :
+      
+
+(* state_behaves_exists: forall (L : Smallstep.semantics) (s : Smallstep.state L), exists beh : program_behavior, state_behaves L s beh *)
+Inductive initial_state (p: program): state -> Prop :=
+  | initial_state_intro: forall b f m0,
+      let ge := Genv.globalenv p in
+      Genv.init_mem p = Some m0 ->
+      Genv.find_symbol ge p.(prog_main) = Some b ->
+      Genv.find_funct_ptr ge b = Some f ->
+      type_of_fundef f = Tfunction Tnil type_int32s cc_default ->
+      initial_state p (Callstate f nil Kstop m0).
+  Definition wf_c_state (ge: Clight.genv) (tr ttr: bundle_trace) (cnts: cnt_ids) id (cst: Clight.state) :=
+    match cst with
+    | State f stmt k_c e le m_c =>
+        wf_counters ge m_c tr cnts /\
+          (exists m_c', Mem.free_list m_c (blocks_of_env ge e) (comp_of f) = Some m_c' /\ wf_c_cont ge m_c' k_c) /\
+          wf_c_stmt ge (comp_of f) cnts id ttr stmt /\
+          (wf_env ge e /\ (not_global_blks (ge) (blocks_of_env2 ge e)) /\ (wf_c_nb ge m_c))
+    | _ => False
+    end.
+  Definition match_state (ge_i: Asm.genv) (ge_c: Clight.genv) (k: meminj) tr cnts pars id (ist: ir_state) (cst: Clight.state) :=
+    match ist, cst with
+    | Some (cur, m_i, k_i), State f _ k_c e le m_c =>
+        (match_genv ge_i ge_c) /\ (match_mem ge_i k m_i m_c) /\
+          (match_cur_fun ge_i ge_c cur f id) /\ (match_find_def ge_i ge_c cnts pars tr) /\
+          (match_cont ge_c tr cnts k_c k_i) /\
+          (match_params pars ge_c ge_i) /\
+          (match_cnts cnts ge_c k)
+    | _, _ => False
+    end.
+
+Variant ir_initial_state (p : Asm.program) : ir_state -> Prop :=
+    ir_initial_state_intro : forall (cur : block) (m0 : mem),
+                             let ge := Genv.globalenv p in
+                             Genv.find_symbol ge (AST.prog_main p) = Some cur ->
+                             (exists f : Asm.function, Genv.find_funct_ptr ge cur = Some (AST.Internal f)) ->
+                             Genv.init_mem p = Some m0 -> ir_initial_state p (Some (cur, m0, [])).
+   Theorem ir_to_clight
+          (ge_i: Asm.genv) (ge_c: Clight.genv)
+          (WFGE: wf_ge ge_i)
+          ist cst
+          ttr cnts pars k id
+          (BOUND: Z.of_nat (Datatypes.length ttr) < Int64.modulus)
+          (WFC: wf_c_state ge_c [] ttr cnts id cst)
+          (MS: match_state ge_i ge_c k ttr cnts pars id ist cst)
+          ist'
+          (STAR: istar (ir_step) ge_i ist ttr ist')
+    :
+    exists cst', star step1 ge_c cst (unbundle_trace ttr) cst'.
+
+
+
+| step_internal_function : forall (f : function) (vargs : list val) (k : cont) (m : mem) (e : env) (le : temp_env) (m1 : mem),
+                             function_entry f vargs m e le m1 ->
+                             step ge function_entry (Callstate (Internal f) vargs k m) E0 (State f (fn_body f) k e le m1)
+Inductive function_entry1 (ge : genv) (f : function) (vargs : list val) (m : mem) (e : env) (le : temp_env) (m' : mem) : Prop :=
+    function_entry1_intro : forall m1 : mem,
+                            list_norepet (var_names (fn_params f) ++ var_names (fn_vars f)) ->
+                            alloc_variables ge (comp_of f) empty_env m (fn_params f ++ fn_vars f) e m1 ->
+                            bind_parameters ge (comp_of f) e m1 (fn_params f) vargs m' ->
+                            le = create_undef_temps (fn_temps f) -> function_entry1 ge f vargs m e le m'.
+Complements.clight_program_has_initial_trace = 
+fun (p : program) (t : trace) => forall beh : program_behavior, program_behaves (semantics1 p) beh -> behavior_prefix t beh
+     : program -> trace -> Prop
+
+End PROOFINIT.
